lawyer/nonblocking/examples/counter.v
@@ -87,7 +87,7 @@ Lemma counter_wfree_spec (l: loc)
   {M} {EM: ExecutionModel heap_lang M} {Σ : gFunctors}
     (OHE : OM_HL_Env OP_HL_WF EM Σ):
   (let _: heap1GS Σ := iem_phys HeapLangEM EM in counter_inv l)
-  ⊢ wait_free_spec_defs.wait_free_method NotStuck (incr l) d_wfr0 5.
+  ⊢ wait_free_spec_defs.wait_free_method NotStuck (incr l) d_wfr0 (fun _ => 5%nat).
 Proof using.
   simpl. rewrite /wait_free_spec_defs.wait_free_method. 
   iIntros "#INV" (τ π q a). iIntros "!> %Φ (CPS & PH) POST".
