lawyer/nonblocking/examples/list_map_adequacy.v
@@ -1,0 +1,45 @@
+From heap_lang Require Import lang notation.
+From lawyer.nonblocking Require Import counter list_map wfree_adequacy wfree_traces.
+
+
+(* TODO: move *)
+Lemma always_returns_impl m etr s1 s2
+  (S12: stuckness_le s1 s2)
+  :
+  always_returns m s1 etr -> always_returns m s2 etr.
+Proof using.
+  rewrite /always_returns. simpl.
+  intros AR [i tpc] **.
+  ospecialize * (AR (trace_context.TraceCtx i tpc)); eauto.
+  destruct AR as [| (->&?)]; [by left| ].
+  destruct s2; try done. by right.
+Qed.
+
+(* TODO: move *)
+Lemma wait_free_impl m C1 C2 s1 s2
+  (C21: forall c, C2 c -> C1 c)
+  (S12: stuckness_le s1 s2):
+  wait_free m C1 s1 -> wait_free m C2 s2.
+Proof using.
+  From trillium.traces Require Import inftraces exec_traces. 
+  rewrite /wait_free. simpl. intros WF ? INIT ??.
+  eapply always_returns_impl; eauto.
+Qed.
+  
+
+Theorem list_map_incr_is_wait_free
+  (l0: loc := Loc 0)
+  : wait_free (λ: "x", hl_list_map_cur (incr l0) "x")%V (counter_is_init_st l0) MaybeStuck.
+Proof using.
+  eapply wait_free_impl with (s1 := MaybeStuck).
+  3: { apply wfree_is_wait_free. eauto. }
+  2: done.
+  Unshelve.
+  2: { unshelve eapply hlm_WF_fix_spec_unsafe.
+       { apply om_wfree_inst.WFS_weaken.
+         apply counter_WF_spec. }
+       2: { simpl. reflexivity. } }
+  simpl. done.
+Qed.
+
+Print Assumptions list_map_incr_is_wait_free.
